common/Linking.v
@@ -297,10 +297,12 @@ Definition link_prog_merge (o1 o2: option (globdef F V)) :=
 
 Definition link_prog :=
   if ident_eq p1.(prog_main) p2.(prog_main)
-  && PTree_Properties.for_all dm1 link_prog_check then
+     && PTree_Properties.for_all dm1 link_prog_check
+     && Policy.eqb p1.(prog_pol) p2.(prog_pol) then
     Some {| prog_main := p1.(prog_main);
             prog_public := p1.(prog_public) ++ p2.(prog_public);
-            prog_defs := PTree.elements (PTree.combine link_prog_merge dm1 dm2) |}
+            prog_defs := PTree.elements (PTree.combine link_prog_merge dm1 dm2);
+            prog_pol := p1.(prog_pol); |}
   else
     None.
 
@@ -311,13 +313,17 @@ Lemma link_prog_inv:
    /\ (forall id gd1 gd2,
          dm1!id = Some gd1 -> dm2!id = Some gd2 ->
          In id p1.(prog_public) /\ In id p2.(prog_public) /\ exists gd, link gd1 gd2 = Some gd)
-  /\ p = {| prog_main := p1.(prog_main);
+   /\ p1.(prog_pol) = p2.(prog_pol)
+   /\ p = {| prog_main := p1.(prog_main);
             prog_public := p1.(prog_public) ++ p2.(prog_public);
-            prog_defs := PTree.elements (PTree.combine link_prog_merge dm1 dm2) |}.
+            prog_defs := PTree.elements (PTree.combine link_prog_merge dm1 dm2);
+            prog_pol := p1.(prog_pol) |}.
 Proof.
   unfold link_prog; intros p E.
   destruct (ident_eq (prog_main p1) (prog_main p2)); try discriminate.
-  destruct (PTree_Properties.for_all dm1 link_prog_check) eqn:C; inv E.
+  destruct (PTree_Properties.for_all dm1 link_prog_check) eqn:C;
+    destruct (Policy.eqb p1.(prog_pol) p2.(prog_pol)) eqn:D;
+    inv E.
   rewrite PTree_Properties.for_all_correct in C.
   split; auto. split; auto.
   intros. exploit C; eauto. unfold link_prog_check. rewrite H0. intros.
@@ -325,6 +331,7 @@ Proof.
   destruct (in_dec peq id (prog_public p2)); try discriminate.
   destruct (link gd1 gd2) eqn:L; try discriminate.
   intuition auto. exists g; auto.
+  split; auto. apply Policy.eq_eqb; auto.
 Qed.
 
 Lemma link_prog_succeeds:
@@ -332,13 +339,16 @@ Lemma link_prog_succeeds:
   (forall id gd1 gd2,
       dm1!id = Some gd1 -> dm2!id = Some gd2 ->
       In id p1.(prog_public) /\ In id p2.(prog_public) /\ link gd1 gd2 <> None) ->
+  p1.(prog_pol) = p2.(prog_pol) ->
   link_prog =
     Some {| prog_main := p1.(prog_main);
             prog_public := p1.(prog_public) ++ p2.(prog_public);
-            prog_defs := PTree.elements (PTree.combine link_prog_merge dm1 dm2) |}.
+            prog_defs := PTree.elements (PTree.combine link_prog_merge dm1 dm2);
+            prog_pol := p1.(prog_pol) |}.
 Proof.
   intros. unfold link_prog. unfold proj_sumbool. rewrite H, dec_eq_true. simpl.
   replace (PTree_Properties.for_all dm1 link_prog_check) with true; auto.
+  apply Policy.eq_eqb in H1; rewrite H1; auto.
   symmetry. apply PTree_Properties.for_all_correct; intros. rename a into gd1.
   unfold link_prog_check. destruct dm2!x as [gd2|] eqn:G2; auto.
   exploit H0; eauto. intros (P & Q & R). unfold proj_sumbool; rewrite ! pred_dec_true by auto.
@@ -346,8 +356,8 @@ Proof.
 Qed.
 
 Lemma prog_defmap_elements:
-  forall (m: PTree.t (globdef F V)) pub mn x,
-  (prog_defmap {| prog_defs := PTree.elements m; prog_public := pub; prog_main := mn |})!x = m!x.
+  forall (m: PTree.t (globdef F V)) pub mn pol x,
+  (prog_defmap {| prog_defs := PTree.elements m; prog_public := pub; prog_main := mn; prog_pol := pol |})!x = m!x.
 Proof.
   intros. unfold prog_defmap; simpl. apply PTree_Properties.of_list_elements.
 Qed.
@@ -378,7 +388,7 @@ Next Obligation.
   intros. transitivity gd2. apply Y. auto. apply R. red; intros; elim H0; auto.
 Defined.
 Next Obligation.
-  apply link_prog_inv in H. destruct H as (L1 & L2 & L3).
+  apply link_prog_inv in H. destruct H as (L1 & L2 & L3 & L4).
   subst z; simpl. intuition auto.
 + red; intros; apply in_app_iff; auto.
 + rewrite prog_defmap_elements, PTree.gcombine, H by auto.
@@ -446,7 +456,8 @@ Definition match_ident_globdef
 Definition match_program_gen (ctx: C) (p1: program F1 V1) (p2: program F2 V2) : Prop :=
   list_forall2 (match_ident_globdef ctx) p1.(prog_defs) p2.(prog_defs)
   /\ p2.(prog_main) = p1.(prog_main)
-  /\ p2.(prog_public) = p1.(prog_public).
+  /\ p2.(prog_public) = p1.(prog_public)
+  /\ p2.(prog_pol) = p1.(prog_pol).
 
 Theorem match_program_defmap:
   forall ctx p1 p2, match_program_gen ctx p1 p2 ->
@@ -671,9 +682,9 @@ Theorem link_match_program:
   linkorder ctx1 ctx -> linkorder ctx2 ctx ->
   exists tp, link tp1 tp2 = Some tp /\ match_program_gen match_fundef match_varinfo ctx p tp.
 Proof.
-  intros. destruct (link_prog_inv _ _ _ H) as (P & Q & R).
-  generalize H0; intros (A1 & B1 & C1).
-  generalize H1; intros (A2 & B2 & C2).
+  intros. destruct (link_prog_inv _ _ _ H) as (P & Q & S & R).
+  generalize H0; intros (A1 & B1 & C1 & D1).
+  generalize H1; intros (A2 & B2 & C2 & D2).
   econstructor; split.
 - apply link_prog_succeeds.
 + congruence.
@@ -683,6 +694,7 @@ Proof.
   exploit Q; eauto. intros (X & Y & gd & Z).
   exploit link_match_globdef. eexact H2. eexact H3. eauto. eauto. eauto.
   intros (tg & TL & _). intuition congruence.
++ congruence.
 - split; [|split].
 + rewrite R. apply PTree.elements_canonical_order'. intros id.
   rewrite ! PTree.gcombine by auto.
@@ -695,7 +707,7 @@ Proof.
   exploit link_match_globdef. eexact H2. eexact H3. eauto. eauto. eauto.
   intros (tg & TL & MG). rewrite Z, TL. constructor; auto.
 + rewrite R; simpl; auto.
-+ rewrite R; simpl. congruence.
++ rewrite R; simpl. split; congruence.
 Qed.
 
 End LINK_MATCH_PROGRAM.
